.

src/program_proof/session/u64ToNat.v
@@ -46,6 +46,10 @@ Instance Similarity_bool : Similarity bool bool :=
 Instance Similarity_nat : Similarity nat nat :=
   @eq nat.
 
+#[global]
+Instance Similarity_Data : Similarity _Data.w _Data.w :=
+  @eq u64.
+
 (** End SIMILARITY. *)
 
 (** Section MONAD. *)
@@ -127,8 +131,6 @@ Class isSuperMonad (M : Type -> Type) `{isMonad M} : Type :=
   ; tryget {A : Type} : M A -> option A
   ; tryget_put_if_true {A : Type} (x : A)
     : tryget (put_if true x) = Some x
-  ; tryget_put_if_false {A : Type} (x : A)
-    : tryget (put_if false x) = None
   ; tryget_pure {A : Type} (x : A)
     : forall z : A, tryget (pure x) = Some z -> x = z
   ; tryget_bind {A : Type} {B : Type} (m : M A) (k : A -> M B)
@@ -136,13 +138,25 @@ Class isSuperMonad (M : Type -> Type) `{isMonad M} : Type :=
   }.
 
 #[global, program]
-Instance Err_isSuperMonad : isSuperMonad Err :=
-  { put_if {A} (guard : bool) (x : A) := (guard, x)
-  ; tryget {A} (m : Err A) := if m.1 then Some m.2 else None
+Instance identity_isSuperMonad : isSuperMonad identity :=
+  { put_if {A} (guard : bool) (x : A) := x
+  ; tryget {A} (m : A) := Some m
   }.
 Next Obligation.
   intros. simpl in *. trivial.
 Qed.
+Next Obligation.
+  intros. simpl in *. congruence.
+Qed.
+Next Obligation.
+  intros. cbn in *. exists m. split; trivial.
+Qed.
+
+#[global, program]
+Instance Err_isSuperMonad : isSuperMonad Err :=
+  { put_if {A} (guard : bool) (x : A) := (guard, x)
+  ; tryget {A} (m : Err A) := if m.1 then Some m.2 else None
+  }.
 Next Obligation.
   intros. simpl in *. trivial.
 Qed.
@@ -164,9 +178,6 @@ Next Obligation.
   intros. simpl in *. trivial.
 Qed.
 Next Obligation.
-  intros. simpl in *. trivial.
-Qed.
-Next Obligation.
   intros. unfold pure in *. simpl in *. congruence.
 Qed.
 Next Obligation.
@@ -175,9 +186,6 @@ Next Obligation.
 Qed.
 
 (** End MONAD. *)
-
-#[global] Arguments bind {M} {isMonad} {A} {B} : simpl never.
-#[global] Arguments pure {M} {isMonad} {A} : simpl never.
 
 (** Section BASIC_CORRES. *)
 
@@ -203,6 +211,148 @@ Definition param3func_corres `{isSuperMonad M} {A : Type} {A' : Type} {B : Type}
   forall c : C, c =~= c' ->
   exists d : D, d =~= d' /\ f a b c = d.
 
+#[global]
+Instance Similarity_u64 : Similarity u64 nat :=
+  fun u => fun n => uint.nat u = n /\ uint.Z u <= CONSTANT - 1.
+
+Module Operation'.
+
+  Record t : Type :=
+    mk
+    { VersionVector : list nat
+    ; Data : nat
+    }.
+
+  Record corres (op : Operation.t) (op' : Operation'.t) : Prop :=
+    Similarity_Operation_INTRO
+    { VersionVector_corres : op.(Operation.VersionVector) =~= op'.(VersionVector)
+    ; Data_corres : op.(Operation.Data) =~= op'.(Data)
+    }.
+
+End Operation'.
+
+#[local] Hint Constructors Operation'.corres : core.
+
+#[global]
+Instance Similarity_Operation : Similarity Operation.t Operation'.t :=
+  Operation'.corres.
+
+Module Message'.
+
+  Record t : Type :=
+    mk
+    { MessageType : nat
+    ; C2S_Client_Id : nat
+    ; C2S_Server_Id : nat
+    ; C2S_Client_OperationType : nat
+    ; C2S_Client_Data : _Data.w
+    ; C2S_Client_VersionVector : list nat
+    ; S2S_Gossip_Sending_ServerId : nat
+    ; S2S_Gossip_Receiving_ServerId : nat
+    ; S2S_Gossip_Operations : list Operation'.t
+    ; S2S_Gossip_Index : nat
+    ; S2S_Acknowledge_Gossip_Sending_ServerId : nat
+    ; S2S_Acknowledge_Gossip_Receiving_ServerId : nat
+    ; S2S_Acknowledge_Gossip_Index : nat
+    ; S2C_Client_OperationType : nat
+    ; S2C_Client_Data : _Data.w
+    ; S2C_Client_VersionVector : list nat
+    ; S2C_Server_Id : nat
+    ; S2C_Client_Number : nat
+    }.
+
+  Record corres (msg : Message.t) (msg' : Message'.t) : Prop :=
+    Similarity_Message_INTRO
+    { MessageType_corres : msg.(Message.MessageType) =~= msg'.(MessageType)
+    ; C2S_Client_Id_corres : msg.(Message.C2S_Client_Id) =~= msg'.(C2S_Client_Id)
+    ; C2S_Server_Id_corres : msg.(Message.C2S_Server_Id) =~= msg'.(C2S_Server_Id)
+    ; C2S_Client_OperationType_corres : msg.(Message.C2S_Client_OperationType) =~= msg'.(C2S_Client_OperationType)
+    ; C2S_Client_Data_corres_corres : msg.(Message.C2S_Client_Data) =~= msg'.(C2S_Client_Data)
+    ; C2S_Client_VersionVector_corres : msg.(Message.C2S_Client_VersionVector) =~= msg'.(C2S_Client_VersionVector)
+    ; S2S_Gossip_Sending_ServerId_corres : msg.(Message.S2S_Gossip_Sending_ServerId) =~= msg'.(S2S_Gossip_Sending_ServerId)
+    ; S2S_Gossip_Receiving_ServerId_corres : msg.(Message.S2S_Gossip_Receiving_ServerId) =~= msg'.(S2S_Gossip_Receiving_ServerId)
+    ; S2S_Gossip_Operations_corres : msg.(Message.S2S_Gossip_Operations) =~= msg'.(S2S_Gossip_Operations)
+    ; S2S_Gossip_Index_corres : msg.(Message.S2S_Gossip_Index) =~= msg'.(S2S_Gossip_Index)
+    ; S2S_Acknowledge_Gossip_Sending_ServerId_corres : msg.(Message.S2S_Acknowledge_Gossip_Sending_ServerId) =~= msg'.(S2S_Acknowledge_Gossip_Sending_ServerId)
+    ; S2S_Acknowledge_Gossip_Receiving_ServerId_corres : msg.(Message.S2S_Acknowledge_Gossip_Receiving_ServerId) =~= msg'.(S2S_Acknowledge_Gossip_Receiving_ServerId)
+    ; S2S_Acknowledge_Gossip_Index_corres : msg.(Message.S2S_Acknowledge_Gossip_Index) =~= msg'.(S2S_Acknowledge_Gossip_Index)
+    ; S2C_Client_OperationType_corres : msg.(Message.S2C_Client_OperationType) =~= msg'.(S2C_Client_OperationType)
+    ; S2C_Client_Data_corres : msg.(Message.S2C_Client_Data) =~= msg'.(S2C_Client_Data)
+    ; S2C_Client_VersionVector_corres : msg.(Message.S2C_Client_VersionVector) =~= msg'.(S2C_Client_VersionVector)
+    ; S2C_Server_Id_corres : msg.(Message.S2C_Server_Id) =~= msg'.(S2C_Server_Id)
+    ; S2C_Client_Number_corres : msg.(Message.S2C_Client_Number) =~= msg'.(S2C_Client_Number)
+    }.
+
+End Message'.
+
+#[local] Hint Constructors Message'.corres : core.
+
+#[global]
+Instance Similarity_Message : Similarity Message.t Message'.t :=
+  Message'.corres.
+
+Module Server'.
+
+  Record t : Type :=
+    mk
+    { Id : nat
+    ; NumberOfServers : nat
+    ; UnsatisfiedRequests : list Message'.t
+    ; VectorClock : list nat
+    ; OperationsPerformed : list Operation'.t
+    ; MyOperations : list Operation'.t
+    ; PendingOperations : list Operation'.t
+    ; GossipAcknowledgements : list nat
+    }.
+
+  Record corres (s : Server.t) (s' : Server'.t) : Prop :=
+    Similarity_Server_INTRO
+    { Id_corres : s.(Server.Id) =~= s'.(Id)
+    ; NumberOfServers_corres : s.(Server.NumberOfServers) =~= s'.(NumberOfServers)
+    ; UnsatisfiedRequests_corres : s.(Server.UnsatisfiedRequests) =~= s'.(UnsatisfiedRequests)
+    ; VectorClock_corres : s.(Server.VectorClock) =~= s'.(VectorClock)
+    ; OperationsPerformed_corres : s.(Server.OperationsPerformed) =~= s'.(OperationsPerformed)
+    ; MyOperations_corres : s.(Server.MyOperations) =~= s'.(MyOperations)
+    ; PendingOperations_corres : s.(Server.PendingOperations) =~= s'.(PendingOperations)
+    ; GossipAcknowledgements_corres : s.(Server.GossipAcknowledgements) =~= s'.(GossipAcknowledgements)
+    }.
+
+End Server'.
+
+#[local] Hint Constructors Server'.corres : core.
+
+#[global]
+Instance Similarity_Server : Similarity Server.t Server'.t :=
+  Server'.corres.
+
+Module Client'.
+
+  Record t : Type :=
+    mk
+    { Id : nat
+    ; NumberOfServers : nat
+    ; WriteVersionVector : list nat
+    ; ReadVersionVector : list nat
+    ; SessionSemantic : nat
+    }.
+
+  Record corres (c : Client.t) (c' : Client'.t) : Prop :=
+    Similarity_Client_INTRO
+    { Id_corres : c.(Client.Id) =~= c'.(Id)
+    ; NumberOfServers_corres : c.(Client.NumberOfServers) =~= c'.(NumberOfServers)
+    ; WriteVersionVector_corres : c.(Client.WriteVersionVector) =~= c'.(WriteVersionVector)
+    ; ReadVersionVector_corres : c.(Client.ReadVersionVector) =~= c'.(ReadVersionVector)
+    ; SessionSemantic_corres : c.(Client.SessionSemantic) =~= c'.(SessionSemantic)
+    }.
+
+End Client'.
+
+#[local] Hint Constructors Client'.corres : core.
+
+#[global]
+Instance Similarity_Client : Similarity Client.t Client'.t :=
+  Client'.corres.
+
 Lemma fold_left_corres `{isSuperMonad M} {A : Type} {A' : Type} {B : Type} {B' : Type} `{Similarity A A'} `{Similarity B B'} (f : A -> B -> A) (f' : A' -> B' -> M A')
   (f_corres : param2func_corres f f')
   : param2func_corres (fold_left f) (fold_left' f').
@@ -216,31 +366,114 @@ Qed.
 
 (** End BASIC_CORRES. *)
 
-#[global]
-Instance Similarity_u64 : Similarity u64 nat :=
-  fun u => fun n => uint.nat u = n /\ uint.Z u <= CONSTANT - 1.
-
-Module Server_u64.
-
-(* TODO: implement Server as u64 with identity monad *)
-
-(* Use SessionPrelude.deleteAt instead of coq_deleteAtIndexOperation, coq_deleteAtIndexMessage. *)
-
-End Server_u64.
-
 Module Server_nat.
 
-(* TODO: implement Server as nat with SuperMonad *)
+  Lemma coq_compareVersionVector_unfold (v1 : list u64) (v2 : list u64) :
+    ServerSide.coq_compareVersionVector v1 v2 =
+    match v1 with
+    | [] => do
+      ret true
+    | h1 :: t1 =>
+      match v2 with
+      | [] => do
+        ret true
+      | h2 :: t2 =>
+        if uint.Z h1 <? uint.Z h2 then do
+          ret false
+        else do
+          ServerSide.coq_compareVersionVector t1 t2
+      end
+    end.
+  Proof.
+    destruct v1; trivial.
+  Qed.
+
+  Fixpoint coq_compareVersionVector `{isSuperMonad M} (v1 : list nat) (v2 : list nat) : M bool :=
+    match v1 with
+    | [] => do
+      ret true
+    | h1 :: t1 =>
+      match v2 with
+      | [] => do
+        ret true
+      | h2 :: t2 => do
+        'b <- coq_compareVersionVector t1 t2;
+        ret ((h2 <=? h1)%nat && b)
+      end
+    end.
+
+  Lemma coq_compareVersionVector_corres `{isSuperMonad M}
+    : param2func_corres (M := M) ServerSide.coq_compareVersionVector coq_compareVersionVector.
+  Proof.
+    intros xs' ys' z' H_OBS xs xs_corres ys ys_corres. revert ys ys' ys_corres z' H_OBS.
+    induction xs_corres as [ | x x' xs xs' x_corres xs_corres IH]; simpl; intros ys ys' ys_corres; destruct ys_corres as [ | y y' ys ys' y_corres ys_corres]; simpl; intros.
+    - exists true; split; s!. apply tryget_pure in H_OBS. ss!.
+    - exists true; split; s!. apply tryget_pure in H_OBS. ss!.
+    - exists true; split; s!. apply tryget_pure in H_OBS. ss!.
+    - specialize (IH ys ys' ys_corres z'). apply tryget_bind in H_OBS. Tac.des.
+      + destruct H_OBS as (b & H_OBS & H_b). apply tryget_pure in H_b. subst z'.
+        exists false; split; trivial. destruct (_ <=? _)%nat as [ | ] eqn: H_OBS'; [rewrite Nat.leb_le in H_OBS' | rewrite Nat.leb_nle in H_OBS'].
+        * do 2 red in x_corres, y_corres. word.
+        * rewrite andb_false_l. reflexivity.
+      + destruct H_OBS as (b & H_OBS & H_b). apply tryget_pure in H_b. subst z'.
+        destruct (_ <=? _)%nat as [ | ] eqn: H_OBS'; [rewrite Nat.leb_le in H_OBS' | rewrite Nat.leb_nle in H_OBS'].
+        * eapply IH. rewrite andb_true_l. exact H_OBS.
+        * do 2 red in x_corres, y_corres. word.
+  Qed.
+
+  Lemma coq_lexicographicCompare_unfold (v1 : list u64) (v2 : list u64) :
+    ServerSide.coq_lexicographicCompare v1 v2 =
+    match v1 with
+    | [] => do
+      ret false
+    | h1 :: t1 =>
+      match v2 with
+      | [] => do
+        ret false
+      | h2 :: t2 =>
+        if uint.Z h1 =? uint.Z h2 then do
+          ServerSide.coq_lexicographicCompare t1 t2
+        else do
+          ret (uint.Z h1 >? uint.Z h2)
+      end
+    end.
+  Proof.
+    destruct v1; trivial.
+  Qed.
+
+  Fixpoint coq_lexicographicCompare `{isSuperMonad M} (v1 : list nat) (v2 : list nat) : M bool :=
+    match v1 with
+    | [] => do
+      ret false
+    | h1 :: t1 =>
+      match v2 with
+      | [] => do
+        ret false
+      | h2 :: t2 =>
+        if uint.Z h1 =? uint.Z h2 then do
+          coq_lexicographicCompare t1 t2
+        else do
+          ret (uint.Z h1 >? uint.Z h2)
+      end
+    end.
+
+  Lemma coq_lexicographicCompare_corres `{isSuperMonad M}
+    : param2func_corres (M := M) ServerSide.coq_lexicographicCompare coq_lexicographicCompare.
+  Proof.
+    intros xs' ys' z' H_OBS xs xs_corres ys ys_corres. revert ys ys' ys_corres z' H_OBS.
+    induction xs_corres as [ | x x' xs xs' x_corres xs_corres IH]; simpl; intros ys ys' ys_corres; destruct ys_corres as [ | y y' ys ys' y_corres ys_corres]; simpl; intros.
+    - exists false; split; s!. apply tryget_pure in H_OBS. ss!.
+    - exists false; split; s!. apply tryget_pure in H_OBS. ss!.
+    - exists false; split; s!. apply tryget_pure in H_OBS. ss!.
+    - specialize (IH ys ys' ys_corres z'). do 2 red in x_corres, y_corres. revert H_OBS; Tac.des; intros; try word.
+      + eapply IH; trivial.
+      + exists true; split; trivial. apply tryget_pure in H_OBS3. do 2 red; trivial.
+      + exists false; split; trivial. apply tryget_pure in H_OBS3. do 2 red; trivial.
+  Qed.
 
 (* Use SessionPrelude.deleteAt instead of coq_deleteAtIndexOperation, coq_deleteAtIndexMessage. *)
 
 End Server_nat.
-
-Module Client_u64.
-
-(* TODO: implement Client as u64 with identity monad *)
-
-End Client_u64.
 
 Module Client_nat.
 
